src/tls/Extensions.fst
@@ -1,3 +1,42 @@
 (* Copyright (C) 2012--2017 Microsoft Research and INRIA *)
 module Extensions
 
+#set-options "--admit_smt_queries true"
+
+let cext_of_custom_aux ((n, e):custom_extension) : clientHelloExtension =
+  CHE_Unknown_extensionType n e
+
+let cext_of_custom el =
+  List.Tot.map cext_of_custom_aux el
+
+let eext_of_custom_aux ((n, e):custom_extension) =
+  EE_Unknown_extensionType n e
+
+let eext_of_custom el =
+  List.Tot.map eext_of_custom_aux el
+
+let custom_of_cext_aux = function
+  | CHE_Unknown_extensionType n e -> Some (n,e)
+  | _ -> None
+
+let custom_of_cext el =
+  List.Tot.choose custom_of_cext_aux el
+
+let custom_of_eext_aux = function
+  | EE_Unknown_extensionType n e -> Some (n,e)
+  | _ -> None
+
+let custom_of_eext el =
+  List.Tot.choose custom_of_eext_aux el
+
+let bindersLen_aux = function
+  | CHE_pre_shared_key psk -> true
+  | _ -> false
+
+let bindersLen che =
+  match List.Tot.find bindersLen_aux che with
+  | None -> 0
+  | Some (CHE_pre_shared_key psk) ->
+    let j = Parsers.OfferedPsks_binders.offeredPsks_binders_size32 psk.binders in
+    UInt32.v j
+
